### 求导法则

## Product rule

$$f(x)=x^a$$

$$f'(x)=a*x^{a-1}$$

##sum rule

$$f(x) = f(a)+f(b)$$

$$f'(x) = f'(a) + f'(b)$$

## 导数的定义

$$ f(x) =  \frac{f(h+x)-f(x)}{h}  $$

当$$x->(x+h)$$无限趋向时候，如果有极限的存在，那么该函数可导

####$$f(x) = x^2$$求导

$$f'(x) = \frac{(x+h)^2-x^2}{h}$$ 

$$f'(x) = \frac{x^2+2xh+h^2-x^2}{h}$$

$$f'(x) = \frac{2xh+h^2}{h}$$

$$f'(x) = {2x+h}$$

$$f'(x) = {2x}$$

#### $$f(x)=x^2$$当$$x=3$$时的导数是多少

$$f'(x) = 2x= 2*3 = 6$$ 

##乘积法则

$$f(x)= h(x)*g(x)$$

$$f'(x) = h'(x)*g(x)+g'(x)*h(x)$$

######可以理解为 一个$$长 = g(x)$$ ,$$高 = h(x)$$ 的长方形，其面积变化率

## 除法法则

$f(x)=h(x)/g(x)$

$f'(x)=h(x)*g(x)^{-1}$

$$f'(x) = h'(x)*g(x)^{-1}+g'(x)^{-1}*h(x)$$

##链式法则

$$f(x) = h(g(x))$$

$$f'(x)=h'(g(x))*g'(x)$$

例如

$$f(x)=(2x+3)^5$$

$$f'(x)=2*5(2x+3)^4$$



$$g(x)=(x^2+2x+3)^8$$

$$g'(x)=(2x+2)*8*(x^2+2x+3)^7$$

