# 指数导数

$$f(x)=a^x$$

$$f'(x)=\frac{a^{x+h}-a^x}{h}$$

$$f'(x)=\frac{a^x*a^h-a^x}{h}$$

$$f'(x)=a^x\frac{(a^h-1)}{h}$$

$$f'(x)=ln(a)*a^x$$

此时，$$a^x的导数几乎等于a^x自己，但后面有一个系数$$

##e的求导

$$f'(e^x)=e^x$$

$$f'(e^{ax})=a*e^{ax}$$



$$f(x)=e^{2x}$$ 求导

$$f'(x)=f'(2x)*f'(e^{2x})$$

$$f'(x)=2*e^{2x}$$

$$f'(x)=2e^{2x}$$

$$f'(x)=l n(2)*2e^{2x}$$



$$2=e^{ln(2)}$$

##证明$$(a^x)^b=a^{a*b}$$

$$f(x)=(a^x)^3$$

$$f(x)=a^x*a^x*a^x$$

$$f(x)=a^{x+x+x}$$

$$f(x)=a^{x*3}$$

##证明$$a^x*a^y=a^{x+y}$$

$$f(x)=a^2*a^3$$

$$f(x)=(a*a)*(a*a*a)$$

$$f(x)=a*a*a*a*a$$

$$f(x)=a^5$$

$$f(x)=a^{2+3}$$

##证明$\frac{1}{x}=x^{-1}$

$1=x^2*\frac{1}{x^2}$

$1=x^2*x^{-2}$

$1=x^{2-2}$

$1=x^0$

##$\frac{1}{x}$求导

$f(x)=\frac{1}{x}$

$f'(x)=\frac{\frac{1}{x+h}-\frac{1}{x}}{h}$

$f'(x)=\frac{\frac{x}{x(x+h)}-\frac{x+h}{x(x+h)}}{h}$

$f'(x)=\frac{\frac{-h}{x(x+h)}}{h}$

$f'(x)=\frac{-h}{x(x+h)}*\frac{1}{h}$

$f'(x)=\frac{-1}{x^2+xh}$

$f'(x)=-\frac{1}{x^2}$

$f'(x)=-x^{-2}$

